almost got lu pivot

programs/LUPivot.fst
@@ -5,22 +5,30 @@ open All
 assume val pivot : #n:pos{n >= 2} -> m:mat n{inv m} ->
   p':mat n{perm p'} & m':mat n{inv m' /\ top_left_nnz m' /\ mat_mul p' m' == m}
 
+// assume val pivot_inverse : #n:pos -> p:mat n -> m:mat n -> m':mat n ->
+//   Lemma (requires perm p /\ mat_mul p m' == m)
+//         (ensures  mat_mul (transpose p) m == m')
+//         [SMTPat (mat_mul (transpose p) m)]
+
+#push-options "--split_queries always"
 let rec lu_pivoting (#n:pos) (m:mat n{inv m}) :
   p:mat n{perm p} & l:mat n{unit_lower l} &
   u:mat n{upper u /\ nnz_diag u /\ mat_mul p m == mat_mul l u} =
-  match n with
-  | 1 -> (|_id_mat, _id_mat, m|)
-  | _ ->
+  match m with
+  | Mat1 _ -> (|_id_mat, _id_mat, m|)
+  | MatN mm mb ma mc ->
     let (|p', m'|) = pivot m in
-    let (|c, a, b, d|) = destruct m' in
+    let (MatN d c a b) = m' in
     let s = schur1 d c a b in
     let (|p, l, u|) = lu_pivoting s in
 
     let lc = vec_scalar_div c a in
     let pd = mat_vec_mul p lc in
-    let l' = augment l pd one zero_rvec in
-    let u' = augment u zero_cvec a b in
-    let p_aug = augment p zero_cvec one zero_rvec in
+    let l' = MatN l pd one zero_rvec in
+    let u' = MatN u zero_cvec a b in
+    let p_aug = MatN p zero_cvec one zero_rvec in
     let p'' = mat_mul p_aug (transpose p') in
 
+    // assert (mat_mul (transpose p') m == m');
     (|p'', l', u'|)
+#pop-options
