programs/Cholesky.fst
@@ -4,12 +4,13 @@ open All
 
 let rec cholesky (#n:pos) (m:mat n{spd m}) :
   l:mat n{lower l /\ pos_diag l /\ mat_mul l (transpose l) == m} =
-  match n with
-  | 1 -> build_mat (sqrt (extract m))
-  | _ ->
-      let (|c, a, b, d|) = destruct m in
+  match m with
+  | Mat1 a -> 
+    assert (pos_diag m);
+    Mat1 (sqrt a)
+  | MatN d c a b ->
       let l11 = sqrt a in
       let l21 = vec_scalar_div c l11 in
       let s = schur1 d c a b in
       let l = cholesky s in
-      augment l l21 l11 zero_rvec
+      MatN l l21 l11 zero_rvec
